\documentclass{beamer} %
\usetheme{CambridgeUS}
\usepackage[latin1]{inputenc}
\usefonttheme{professionalfonts}
\usepackage{times}
\usepackage{amsmath}
\usepackage{verbatim}
\usepackage{pst-node}
\usepackage{tikz-cd} 

\newcommand\blfootnote[1]{%
  \begingroup
  \renewcommand\thefootnote{}\footnote{#1}%
  \addtocounter{footnote}{-1}%
  \endgroup
}

\author{Joe Isaacs}
\title{Monad and Comonads}
\institute{Churchill CompSci talks}
\date{\today}

\begin{document}

\begin{frame}
  \titlepage
\end{frame}

\section{Type Classes in Haskell}

\begin{frame}[fragile]\frametitle{Type classes}
\begin{verbatim}
class Eq where
  (==) :: a -> a -> Bool
\end{verbatim}

\begin{verbatim}
instance Eq Integer where
  (==) a b = intEq a b

triEq :: (Eq a) -> a -> a -> a
triEq a b c = (a==b) && (a==c) && (b==c)
\end{verbatim}
\end{frame}

\section{Functor}

\begin{frame}{Functor}
  \begin{itemize}
    \item Functors $F$ will map from a catagory $C$ to a catagory $D$ written as 
      \[ F : C \rightarrow D \]

    \item An object $A$ in $C$ will be mapped to $F(A)$ in $D$

    \item Functors map morphisms $f : A \rightarrow B$ to $F(f) : F(A) \rightarrow F(B)$

    \item $F(id_A) = id_{F(A)}$ where $id_A : A \rightarrow A$ and 
      $id_{F(A)} : F(A) \rightarrow F(A)$

    \item $F(f \circ g) = F(f) \circ F(g) $ (functors distribute over morphism composition).
  \end{itemize}
\end{frame}

\begin{frame}[fragile]\frametitle{Functor in Haskell}
  \begin{itemize}
    \item A function $F$ will map $f : A \rightarrow B$ to $F(f) : F(A) \rightarrow F(B)$
     
    \item 
\begin{verbatim}
class Functor f where
   fmap :: (a -> b) -> f a -> f b
\end{verbatim}

  \item $id_A = \texttt{id :: a -> a}$

  \item $id_{F(A)} = \texttt{fmap id :: f a -> f a}$ 

  \item $F(h\circ g) = \texttt{fmap (h.g) :: f a -> f c}$

  \item $F(h) \circ F(g) = \texttt{fmap h . fmap g :: f a -> f c}$
  \end{itemize}
  where $\circ = \texttt{(.)}$, $h = \texttt{h :: b -> c}$,  $g = \texttt{g :: a -> b}$ and
  $F = \texttt{Functor f}$
\end{frame}

\begin{frame}[fragile]\frametitle{Functor example \texttt{Maybe}}
\begin{verbatim}
data Maybe a = Nothing | Just a
instance Functor Maybe where
  fmap f (Just x) = Just (f x)
  fmap _ Nothing    = Nothing
\end{verbatim}
\begin{itemize}
  \item Must check $F(id_A) = id_{F(A)}$
\begin{verbatim}
  fmap id x
case (x == Just a)
  fmap id (Just a) a === Just (id a) === Just a
case (x == Nothing)
  fmap id Nothing === Nothing

==> fmap id = id
\end{verbatim}
\end{itemize}
\end{frame}

\begin{frame}[fragile]\frametitle{Functor example \texttt{Maybe}}
Check $F(f \circ g) = F(f) \circ F(g)$
\begin{verbatim}
case (Just a)
      fmap (f.g) (Just a) 
  === Just ((f.g) a)
  === Just (f (g a))

      (fmap f . fmap g) (Just a) 
  === fmap f (fmap g (Just a)) 
  === fmap f (Just (g a))
  === Just (f(g a))
case (Nothing)
  fmap (f.g) Nothing == Nothing
      fmap f . fmap g Nothing 
  === fmap f Nothing
  === Nothing
\end{verbatim}
\end{frame}

\section{Monad}

\begin{frame}{Monad}
  \begin{itemize}
    \item Defined by $(M,\mathit{join},\mathit{unit})$

    \item $M$ is the monad and also a functor

    \item $\mathit{join}$ is the transformation $M (M a) \rightarrow M a$ which satifies
      \[ \mathit{join} \circ M (\mathit{join}) = \mathit{join} \circ \mathit{join}  \]
      and \[ \mathit{join} \circ M(M(f)) = M(f) \circ \mathit{join} \]
    
    \item $\mathit{unit}$ is the transformation $a \rightarrow M a$ which satifies 
      \[ \mathit{join} \circ M \mathit{unit} = \mathit{join} \circ \mathit{unit}  = I_M \] where $I_M$ is a transformation
      from $M \rightarrow M$ and \[ \mathit{unit} \circ f = M(f) \circ \mathit{unit} \]


  \end{itemize}
\end{frame}

\begin{frame}[fragile]\frametitle{Monad in Haskell}
We have seen the catagorical definition of monads above, this could be a
Haskell implementation.
\begin{verbatim}
class Functor m => Monad m where
  unit :: a -> m a
  join  :: m a -> (a -> m b) -> m b
\end{verbatim}
\begin{itemize}
  \item $\mathit{unit} = \texttt{unit}$

  \item $\mathit{join} = \texttt{join}$
  \item The monad laws can now be written in Haskell as:
\begin{verbatim}
join . fmap join     = join . join
join . fmap unit     = join . unit    = id
unit . f             = fmap f . unit
join . fmap (fmap f) = fmap f . join
\end{verbatim}
\end{itemize}
\end{frame}

\begin{frame}[fragile]\frametitle{What do the laws mean?}
We can explain all the laws
\begin{verbatim}
join . fmap join = join . join
\end{verbatim}
with commutative diagrams, here is the first:

\[ 
\begin{tikzcd}
M^3 \arrow{r}{\mathit{join}} \arrow[swap]{d}{M(\mathit{join})} & M^2 \arrow{d}{\mathit{join}} \\
M^2 \arrow{r}{\mathit{join}} & M
\end{tikzcd}
\]
\end{frame}

\begin{frame}[fragile]\frametitle{How Monads are really implemented in Haskell}
\begin{itemize}
  \item Haskell implements monad in different but equivalent way:

\begin{verbatim}
class Functor m => Monad m where
  return :: a -> m a
  (>>=)  :: m a -> (a -> m b) -> m b
  fail   :: String -> m a
\end{verbatim}
\item $\texttt{return} = \texttt{unit}$

\item \texttt{(>>=)} (pronounced bind) can be derived form \texttt{unit} and \texttt{fmap}:

\begin{verbatim}
join x = x >>= id

x >>= f = join (fmap f x)
\end{verbatim}
\end{itemize}
\end{frame}

\begin{frame}[fragile]\frametitle{Monad laws using \texttt{(>>=)}}
  \begin{itemize}
    \item 
\begin{verbatim}
m >>= return = m
return m >>= f = f m
(m >>= f) >>= g = m >>= (\x -> f x >>= g)
\end{verbatim}
These are left identity, right identity and associativity
  \item It can also be show that these three monad laws are equivalent to the four monad laws
    stated previously.
\end{itemize}
\end{frame}

\begin{frame}[fragile]\frametitle{Example: \texttt{Maybe}}
\begin{verbatim}
instance Monad Maybe where
  return        = Just
  fail _        = Nothing
  Just x  >>= f = f x
  Nothing >>= _ = Nothing
\end{verbatim}
The Maybe instance of Monad must also follow the monad laws stated previously.
\begin{verbatim}
m >>= return = m

Just x >>= return === return x === Just x

Nothing >>= return === Nothing
\end{verbatim}
\end{frame}

\section{Monad uses}

\begin{frame}[fragile]\frametitle{Computations with possible errors}
\begin{verbatim}
computeB ::            a -> Maybe b
computeC ::            b -> Maybe c

compute  ::            a -> Maybe c
compute a = case computeB of
              Just b  -> computeC b
              Nothing -> Nothing
\end{verbatim}
\end{frame}

\begin{frame}[fragile]\frametitle{Computations with possible errors Cont.}
\begin{verbatim}
computeB :: Monad m => a -> m     b
computeC :: Monad m => b -> m     c

compute  :: Monad m => a -> m     c
compute a = computeB a >>= computeC
\end{verbatim}
\end{frame}

\begin{frame}[fragile]\frametitle{do-notation}
\begin{verbatim}
do x                 ==> \usepackage{biblatex}x

do let y = z         ==> let y = z in do x
   x

do y <- z           ==> z >>= \y -> do x
   x

do y                ==> y >>= \_ -> do x
   x

compute :: a -> Maybe c
compute a = 
  do b <- computeB a
     computeC
\end{verbatim}
\end{frame}

\begin{frame}[fragile]\frametitle{Monoid}
    A monoid is an object $M$ with two morphisms $\mathit{mult}: M \oplus M \rightarrow M$ and $\mathit{unit} : I \rightarrow M$. 

    Where both \[\mathit{unit} \circ M = M = M \circ \mathit{unit} \text{ (left and right
        identity)}\] and
    \[ \mathit{mult} \circ (\mathit{mult} \circ \mathit{mult}) = (\mathit{mult} \circ \mathit{mult})
    \circ \mathit{mult} \text{ (associativity)} \]

\begin{verbatim}
class Monoid a where 
  mzero   :: a
  mappend :: a -> a -> a
\end{verbatim}
$\mathit{unit} = \tex\usepackage{biblatex}ttt{mzero}$ and $\mathit{mult} = \texttt{mappend}$
\end{frame}

\begin{frame}[fragile]\frametitle{Writer Monad Motivation: Logging}
  \begin{itemize}
    \item Want to store order set of stages throughout a computation.
\begin{verbatim}
addOne :: Int -> Int -> [String]
addOne x = (x+1,["Added 1 to " ++ show x])

applyLogger :: Monoid m => 
               (v,m) -> (v -> (o, m)) -> (o,m)
applyLogger (input,log) f = (o, log `mappend` l)
  where (o,l) = f input

addOne 0 `applyLogger` addOne 
`applyLogger` addone

> (3,["Added 1 to 0"
     ,"Added 1 to 1","Added 1 to 2"])
\end{verbatim}
  \end{itemize}
\end{frame}

\begin{frame}[fragile]\frametitle{Write Monad}
\begin{verbatim}
newtype Writer w a = Writer { runWriter :: (a,w) }

instance (Monoid w) => Monad (Writer w) where
  return x = writer (x,mempty)
  (Writer (x,v)) >>= f = let (Writer (y,v')) = f x 
                         in Writer (y,v `mappend` v')
\end{verbatim}
\end{frame}

\begin{frame}[fragile]\frametitle{Logging with the Write Monad}
\begin{verbatim}

logNumber :: Int -> Writer [String] Int
logNumber x = Writer (x, ["Recored " ++ (show x))

runWriter 
(do a <- logNumber 10
   b <- logNumber 11
   return (a*b))
> (110,["Recored 10", "Recored 11"])
\end{verbatim}
\end{frame}

\section{Comonad}

\begin{frame}[fragile]\frametitle{Comonad}
  \begin{itemize}
    \item Dual of a monad


    \item Remember Monad has two morphisms
      \begin{itemize}
        \item $\mathit{unit} : a \rightarrow M a$
        \item $\mathit{join} : M (M a) \rightarrow M a$
      \end{itemize}

    \item A comonad $C$ defines two transformations:
      \begin{itemize}
        \item $\mathit{extract} : C a \rightarrow a$ 

        \item $\mathit{duplicate}  : C a \rightarrow C (C a)$
      \end{itemize}
    \item Satisfying three laws:
      \begin{itemize}
        \item $\mathit{extend} \circ \mathit{duplicate} = I_C$
        \item $C(\mathit{extract}) \circ \mathit{duplicate} = I_C$
        \item $C(\mathit{duplicate}) \circ \mathit{duplicate} = \mathit{duplicate}
          \circ \mathit{duplicate}$
      \end{itemize}
    \item Is also a functor.
  \end{itemize}
\end{frame}

\begin{frame}[fragile]\frametitle{Comonad in Haskell}
\begin{verbatim}
class Functor w => Comonad w where
  extract :: w a -> a
  extend  :: (w a -> b) -> w a -> w b
\end{verbatim}
we can define extend as \texttt{extend f = fmap f.duplicate}

This must also obey the laws:
\begin{verbatim}
extend extract      = id
extract . extend f  = f
extend f . extend g = extend (f. extend g)
\end{verbatim}
\end{frame}

\begin{frame}[fragile]\frametitle{Array filters are comonads}

\begin{verbatim}
data CArray i a = CA (Array i a) i deriving Show

instance Ix i => Comonad (CArray i) where
  extract (CA arr c) = arr!c
  extend f (CA x c)  =
    let  es' = map (\i -> (i,f(CA x i))) (indices x)
    in   CA (array (bounds x) es') c

laplace1D :: Num a => CArray Integer a -> a
laplace1D a = (a ? (-1)) + (a ? 1)  - 2 * (a ? 0)
\end{verbatim}
\texttt{(?)} will try to get the value at \texttt{i+i'} of the value \texttt{a} 
where \texttt{(CA a i)} 

\blfootnote{Example from A Notation for Comonads by Dominic Orchard and Alan Mycroft}
\end{frame}


\end{document}
